Work on the program logic soundness

src/MicroSail/Sep/Soundness/HoareSound.v
@@ -1,5 +1,7 @@
 Require Import Coq.Program.Tactics.
+Require Import Coq.Program.Equality.
 Require Import FunctionalExtensionality.
+Require Import Equations.Equations.
 
 Require Import MicroSail.Syntax.
 Require Import MicroSail.Environment.
@@ -7,38 +9,574 @@ Require Import MicroSail.SmallStep.Inversion.
 Require Import MicroSail.Sep.Logic.
 Require Import MicroSail.Sep.Spec.
 Require Import MicroSail.Sep.Hoare.
+Require Import MicroSail.Sep.Model.Disjoint.
 
 Module HoareSound
        (Import typekit : TypeKit)
        (Import termkit : TermKit typekit)
        (Import progkit : ProgramKit typekit termkit)
        (Import assertkit : AssertionKit typekit termkit progkit)
-       (Import heapkit : HeapKit typekit termkit progkit assertkit).
+       (Import contractkit : SymbolicContractKit typekit termkit progkit assertkit)
+       (Import heapkit : HeapKit typekit termkit progkit assertkit contractkit).
   Module SSI := Inversion typekit termkit progkit.
   Import SSI.
   Import SS.
 
-  Module PL := ProgramLogic typekit termkit progkit assertkit heapkit.
+  Module PL := ProgramLogic typekit termkit progkit assertkit contractkit heapkit.
   Import PL.
 
-Section Soundness.
-  Context {A : Type} {Logic : Heaplet A} (Valid : A -> Prop).
+  Module Model := Disjoint typekit termkit progkit assertkit contractkit heapkit.
+  Import Model.
 
-  Open Scope logic.
+  Section Soundness.
+
+    Open Scope logic.
+
+    (* forall (γ γ' : RegStore) (μ μ' : Memory) (δ δ' : LocalStore Γ) (s' : Stm Γ σ), *)
+    (*   ⟨ γ, μ, δ, s ⟩ --->* ⟨ γ', μ', δ', s' ⟩ -> Final s' -> *)
+    (*   forall (POST : Lit σ -> LocalStore Γ -> RegStore -> Prop), *)
+    (*     WLP s POST δ γ -> ResultNoFail s' (fun v => POST v δ' γ'). *)
+
+    Definition Total (h : Heap) : Prop :=
+      forall σ r, exists v, h σ r = Some v.
+
+    Definition heap (rs : RegStore) : Heap :=
+      fun _ r => Some (read_register rs r).
+
+    Lemma RegStoreIsTotal (rs : RegStore) : Total (heap rs).
+    Proof.
+      intros σ r.
+      exists (read_register rs r).
+      now unfold heap.
+    Qed.
+
+    Local Ltac sound_steps_inversion :=
+      repeat
+        match goal with
+        | [ H: ResultNoFail _ _ |- _ ] =>
+          apply result_no_fail_inversion in H; destruct_conjs; subst
+        | [ H: ⟨ _, _, _, ?s ⟩ ---> ⟨ _, _, _, _ ⟩ |- _ ] =>
+          microsail_stm_primitive_step s; dependent destruction H
+        | [ H: ⟨ _, _, _, ?s ⟩ --->* ⟨ _, _, _, ?t ⟩, HF: Final ?t |- _ ] =>
+          first
+            [ microsail_stm_primitive_step s; dependent destruction H; cbn in HF
+            | match head s with
+              | @stm_call'   => apply (steps_inversion_call'  HF) in H
+              | @stm_let     => apply (steps_inversion_let    HF) in H
+              | @stm_let'    => apply (steps_inversion_let'   HF) in H
+              | @stm_seq     => apply (steps_inversion_seq    HF) in H
+              | @stm_assign  => apply (steps_inversion_assign HF) in H
+              | @stm_bind    => apply (steps_inversion_bind   HF) in H
+              end; destruct_conjs
+            ]
+        | _ => progress (cbn in *)
+                        end.
+
+  Import EnvNotations.
+
+  Local Ltac sound_simpl :=
+    repeat
+      match goal with
+      | [ H: True |- _ ] => clear H
+      | [ H: False |- _ ] => destruct H
+      | [ H: Env _ (ctx_snoc _ _) |- _ ] =>
+        dependent destruction H
+      | [ H: Env _ ctx_nil |- _ ] =>
+        dependent destruction H
+      | [ H: context[env_drop _ (_ ►► _)]|- _] =>
+        rewrite env_drop_cat in H
+      | [ _: context[match eval ?e ?δ with _ => _ end] |- _ ] =>
+        destruct (eval e δ)
+      | _ => progress (cbn in *; destruct_conjs; subst)
+      end.
+
+    (* Lemma sound {Γ σ} (s : Stm Γ σ) : *)
+    (*   forall (γ γ' : RegStore) (μ μ' : Memory) (δ δ' : LocalStore Γ) (s' : Stm Γ σ), *)
+    (*   ⟨ γ, μ, δ, s ⟩ --->* ⟨ γ', μ', δ', s' ⟩ -> Final s' -> *)
+    (*   forall (PRE : HProp) (POST : Lit σ -> LocalStore Γ -> HProp) *)
+    (*     (triple : δ ⊢ ⦃ PRE ⦄ s ⦃ POST ⦄) *)
+    (*     (γframe γfocus : Heap), *)
+    (*       split (heap γ) γframe γfocus -> *)
+    (*       PRE γfocus -> *)
+    (*       (exists (γfocus' : Heap), *)
+    (*         ResultNoFail s' (fun v => POST v δ' γfocus')). *)
+    (* Proof. *)
+    (*   intros. *)
+    (*   generalize dependent γfocus. *)
+    (*   generalize dependent γframe. *)
+    (*   generalize dependent γ. *)
+    (*   induction s; intros. *)
+    (*   3:{ cbn in *. *)
+    (*       sound_steps_inversion. *)
+
+  (*   Lemma sound_stm_seq {Γ σ} (s : Stm Γ σ) *)
+  (*         (s_eq : exists τ s1 s2 *)
+  (* (IHs1 : forall (s' : Stm Γ τ) (γ γ' : RegStore) (μ μ' : Memory) *)
+  (*          (δ δ' : LocalStore Γ) (PRE : HProp) (POST : Lit τ -> LocalStore Γ -> HProp), *)
+  (*        δ ⊢ ⦃ PRE ⦄ s1 ⦃ POST ⦄ -> *)
+  (*        Final s' -> *)
+  (*        ⟨ γ, μ, δ, s1 ⟩ --->* ⟨ γ', μ', δ', s' ⟩ -> *)
+  (*        forall γfocus : Heap, *)
+  (*        PRE γfocus -> *)
+  (*        forall γframe : Heap, *)
+  (*        split (heap γ) γframe γfocus -> *)
+  (*        exists γframe' γfocus' : Heap, *)
+  (*          split (heap γ') γframe' γfocus' /\ *)
+  (*          ResultNoFail s' (fun v : Lit τ => POST v δ' γfocus')) *)
+  (* (IHs2 : forall (s' : Stm Γ σ) (γ γ' : RegStore) (μ μ' : Memory) *)
+  (*          (δ δ' : LocalStore Γ) (PRE : HProp) (POST : Lit σ -> LocalStore Γ -> HProp), *)
+  (*        δ ⊢ ⦃ PRE ⦄ s2 ⦃ POST ⦄ -> *)
+  (*        Final s' -> *)
+  (*        ⟨ γ, μ, δ, s2 ⟩ --->* ⟨ γ', μ', δ', s' ⟩ -> *)
+  (*        forall γfocus : Heap, *)
+  (*        PRE γfocus -> *)
+  (*        forall γframe : Heap, *)
+  (*        split (heap γ) γframe γfocus -> *)
+  (*        exists γframe' γfocus' : Heap, *)
+  (*          split (heap γ') γframe' γfocus' /\ *)
+  (*          ResultNoFail s' (fun v : Lit σ => POST v δ' γfocus')), *)
+  (*             s = @stm_seq Γ τ s1 σ s2)  : *)
+  (*     forall (γ γ' : RegStore) (μ μ' : Memory) (δ δ' : LocalStore Γ) (s' : Stm Γ σ), *)
+  (*     ⟨ γ, μ, δ, s ⟩ --->* ⟨ γ', μ', δ', s' ⟩ -> Final s' -> *)
+  (*     forall (PRE : HProp) (POST : Lit σ -> LocalStore Γ -> HProp) *)
+  (*       (triple : δ ⊢ ⦃ PRE ⦄ s ⦃ POST ⦄) *)
+  (*       (γframe γfocus : Heap), *)
+  (*         split (heap γ) γframe γfocus -> *)
+  (*         PRE γfocus -> *)
+  (*         exists (γframe' γfocus' : Heap), *)
+  (*           split (heap γ') γframe' γfocus' /\ *)
+  (*           ResultNoFail s' (fun v => POST v δ' γfocus'). *)
+  (*     Proof. *)
+  (*       intros γ γ' μ μ' δ δ' s' Hsteps Hfinal PRE POST triple γframe γfocus Hsplit_γ Hpre. *)
+  (*       inversion s_eq as [τ [s1 [s2 [IHs1 [ IHs2 eq]]]]]. subst. clear s_eq. *)
+  (*       sound_steps_inversion. *)
+  (*       sound_simpl. *)
+  (*       rename Hsteps into γ0. *)
+  (*       induction triple. *)
+  (*       (* consequence *) *)
+  (*       - destruct (IHtriple s1 s2 δ' s' H0 H1 H2 H3 H4 H5 H6 Hfinal *)
+  (*                   (H7 γfocus Hpre) IHs1 IHs2) as [γframe' [γfocus' [IHsplit IHresult]]]. *)
+  (*            exists γframe', γfocus'. *)
+  (*            split. *)
+  (*            ** apply IHsplit. *)
+  (*            ** destruct s'; cbn in *; try congruence. *)
+  (*               apply (H8 _ _ _ IHresult). *)
+  (*       (* frame *) *)
+  (*       - admit. *)
+  (*       - dependent destruction H1; *)
+  (*         cbn in *; *)
+  (*         sound_steps_inversion; *)
+  (*         sound_simpl. *)
+  (*         + exists γframe, γfocus. *)
+  (*           Abort. *)
+(*           + (* specialize (step_trans H5 H6) as H7. *) *)
+(*             specialize (IHs1 (stm_lit τ l) γ γ0 μ μ0 δ δ0 P6 (fun _ => Q5) t7 *)
+(*                              (ltac:(now cbn)) H2 γfocus HPRE γframe Hsplit_γ). *)
+(*             inversion IHs1 as [γframe' [γfocus' [Hsplit_γ' HQ]]]. clear IHs1. *)
+(*             cbn in HQ. *)
+(*             specialize (IHs2 s' γ0 γ' μ0 μ' δ0 δ' (Q5 δ0) R1 (t8 δ0) HFinal_s' *)
+(*                              H6 γfocus' HQ γframe' Hsplit_γ'). *)
+(*             apply IHs2. *)
+
+
+(* dependent destruction H1; *)
+(*           cbn in *; *)
+(*           sound_steps_inversion; *)
+(*           sound_simpl. *)
+(*           + *)
+(* Abort. *)
+    (*         specialize (IHs1 (stm_lit τ l) γ γ0 μ μ0 δ δ0 P6 (fun _ => Q5) t7 *)
+    (*                          (ltac:(now cbn)) H2 γfocus HPRE γframe Hsplit_γ). *)
+    (*         inversion IHs1 as [γframe' [γfocus' [Hsplit_γ' HQ]]]. clear IHs1. *)
+    (*         cbn in HQ. *)
+    (*         specialize (IHs2 s' γ0 γ' μ0 μ' δ0 δ' (Q5 δ0) R1 (t8 δ0) HFinal_s' *)
+    (*                          H6 γfocus' HQ γframe' Hsplit_γ'). *)
+    (*         apply IHs2. *)
+    (*     intros. *)
+
+
+    Lemma sound {Γ σ} (s : Stm Γ σ) :
+      forall (γ γ' : RegStore) (μ μ' : Memory) (δ δ' : LocalStore Γ) (s' : Stm Γ σ),
+      ⟨ γ, μ, δ, s ⟩ --->* ⟨ γ', μ', δ', s' ⟩ -> Final s' ->
+      forall (PRE : HProp) (POST : Lit σ -> LocalStore Γ -> HProp)
+        (triple : δ ⊢ ⦃ PRE ⦄ s ⦃ POST ⦄)
+        (γframe γfocus : Heap),
+          split (heap γ) γframe γfocus ->
+          PRE γfocus ->
+          exists (γframe' γfocus' : Heap),
+            split (heap γ') γframe' γfocus' /\
+            ResultNoFail s' (fun v => POST v δ' γfocus').
+    Proof.
+      (* intros. *)
+      (* generalize dependent γframe. *)
+      (* generalize dependent γfocus. *)
+      (* generalize dependent H. *)
+      (* generalize dependent H0. *)
+      (* generalize dependent POST. *)
+      (* generalize dependent PRE. *)
+      (* revert s' γ γ' μ μ' δ δ'. *)
+      induction s.
+      (* stm_lit *)
+      * intros γ γ' μ μ' δ δ' s' Hsteps Hfinal PRE POST triple γframe γfocus Hsplit_γ Hpre.
+        sound_steps_inversion.
+        sound_simpl.
+        dependent induction triple.
+        (* rule_consequence *)
+        + specialize (IHtriple l P' Q' eq_refl JMeq_refl JMeq_refl eq_refl JMeq_refl).
+          specialize (IHtriple γframe γfocus Hsplit_γ (H γfocus Hpre)).
+          inversion IHtriple as [γframe' [γfocus' [Hsplit_γ' HQ']]].
+          clear IHtriple.
+          exists γframe', γfocus'.
+          intuition.
+        (* rule_frame *)
+        + inversion Hpre as [γl [γr [Hsplit_γfocus [HR HP]]]].
+          clear Hpre.
+          specialize (IHtriple l P Q eq_refl JMeq_refl JMeq_refl eq_refl JMeq_refl).
+          destruct (split_assoc_r (heap γ) γframe γfocus γl γr Hsplit_γ Hsplit_γfocus)
+          as [γ0 [Hsplit_γ0r Hsplit_γframer]].
+          specialize (IHtriple γ0 γr Hsplit_γ0r HP).
+          inversion IHtriple as [γframe' [γfocus' [Hsplit_γ' HQ']]]. clear IHtriple.
+          exists γframe', γfocus'.
+          split.
+          ++ apply Hsplit_γ'.
+          ++ cbn in *.
+             exists γl, γr.
+             admit.
+        (* rule_stm_lit *)
+        + exists γframe, γfocus.
+          split.
+          ++ apply Hsplit_γ.
+          ++ now cbn in *.
+     (* stm_exp *)
+     *
+
+
+
+
+        exists γframe, γfocus.
+        split.
+        ** apply Hsplit_γ.
+        **
+           +
+
+               triple Hfinal
+                  γfocus HPRE γframe Hsplit_γ.
+      10:{
+        intros s' γ γ' μ μ' δ δ' PRE POST triple Hfinal Hsteps
+                  γfocus HPRE γframe Hsplit_γ.
+        sound_steps_inversion.
+        sound_simpl.
+        rename Hsteps into γ0.
+        dependent elimination triple.
+        3:{
+        dependent induction triple.
+        3:{ simplify_IH_hyps.
+            simpl_JMeq.
+            simpl_depind.
+
+      10:{ intros γ γ' μ μ' δ δ' s' Hsteps Hfinal PRE POST triple
+                  γframe γfocus Hsplit_γ HPRE.
+           sound_steps_inversion.
+           sound_simpl.
+           rename Hsteps into γ0.
+           induction triple.
+           (* dependent elimination triple. *)
+           * specialize (IHtriple s1 s2 IHs1 IHs2 δ' s' H0 H1 H2 H3 H4 H5 H6 Hfinal
+                       (H7 γfocus HPRE)) as [γframe' [γfocus' [IHsplit IHresult]]].
+             exists γframe', γfocus'.
+             split.
+             ** apply IHsplit.
+             ** destruct s'; cbn in *; try congruence.
+                apply (H8 _ _ _ IHresult).
+           * admit.
+           * dependent destruction H1;
+             cbn in *;
+             sound_steps_inversion;
+             sound_simpl.
+             specialize (IHs2 γ0 γ' μ0 μ' δ0 δ' s' H6 Hfinal).
+
+             (Q5 δ0) R1 (t8 δ0) HFinal_s'
+                            H6 γfocus' HQ γframe' Hsplit_γ').
+
+             sound_steps_inversion.
+             sound_simpl.
+
+             +
+               (* specialize (step_trans H5 H6) as H7. *)
+                 specialize (IHs1 (stm_lit τ l0) γ γ0 μ μ0 δ δ0
+                                  ⊤ (fun v δ' => !!(l0 = v /\ δ = δ'))
+                                  ). P6 (fun _ => Q5) t7
+                            (ltac:(now cbn)) H2 γfocus HPRE γframe Hsplit_γ).
+                 inversion IHs1 as [γframe' [γfocus' [Hsplit_γ' HQ]]]. clear IHs1.
+                 cbn in HQ.
+                 specialize (IHs2 s' γ0 γ' μ0 μ' δ0 δ' (Q5 δ0) R1 (t8 δ0) HFinal_s'
+                            H6 γfocus' HQ γframe' Hsplit_γ').
+                 apply IHs2.
+  (* specialize (IHs1 (stm_lit τ l) γ γ0 μ μ0 δ δ0 P6 (fun _ => Q5) t7 *)
+  (*                           (ltac:(now cbn)) H2 γfocus HPRE γframe Hsplit_γ). *)
+  (*                inversion IHs1 as [γframe' [γfocus' [Hsplit_γ' HQ]]]. clear IHs1. *)
+  (*                cbn in HQ. *)
+  (*                specialize (IHs2 s' γ0 γ' μ0 μ' δ0 δ' (Q5 δ0) R1 (t8 δ0) HFinal_s' *)
+  (*                           H6 γfocus' HQ γframe' Hsplit_γ'). *)
+  (*                apply IHs2. *)
+               + admit. }
+
+
+                 sound_steps_inversion.
+                 sound_simpl.
+
+               + cbn in *.
+                 sound_steps_inversion.
+                 sound_simpl.
+
+                 dependent destruction t7.
+
+
+
+
+
+
+
+
+      induction .
+      9:{
+        intros HFinal_s' Hsteps γfocus HP γframe Hsplit_γ.
+        sound_steps_inversion.
+        sound_simpl.
+        rename Hsteps into γ0.
+
+
+
+      (* consequence *)
+      - intros γfocus HP γframe Hsplit_γ.
+        destruct (IHtriple δ' s' H H0 γfocus (H1 γfocus HP) γframe Hsplit_γ)
+          as [γfocus' IH].
+        exists γfocus'.
+        destruct (result_no_fail_inversion _ _ IH) as [v [s'eq HQ']].
+        subst.
+        unfold ResultNoFail.
+        apply (H2 _ _ γfocus' HQ').
+      (* frame *)
+      - intros γfocus HRP γframe Hsplit_γ.
+        inversion HRP as [γl [γr [Hsplit_γfocus [HR HP]]]].
+        destruct (split_assoc_r (heap γ) γframe γfocus γl γr Hsplit_γ Hsplit_γfocus)
+          as [γ0 [Hsplit_γ0r Hsplit_γframer]].
+        destruct (IHtriple δ' s' H H0 γr HP γ0 Hsplit_γ0r) as [γfocus' IH].
+        (* stuck: do we need some sort of connection between γfocus and γfocus'? *)
+        admit.
+      (* rule_stm_lit *)
+      - intros. cbn in *.
+        sound_steps_inversion.
+        now exists γfocus.
+      (* rule_stm_exp_forwards *)
+      - intros.
+        sound_steps_inversion; try contradiction.
+        exists γfocus. intuition.
+      (* rule_stm_exp_backwards *)
+      - admit.
+      (* rule_stm_let *)
+      - intros.
+      (*    sound_steps_inversion. *)
+      (*    sound_simpl. *)
+      (*    cbn in *. *)
+      (*    dependent destruction s'. *)
+      (*    + cbn in *. *)
+      (*      dependent destruction H7. *)
+      (*      ++ cbn in *. *)
+      (*         specialize (H2 l0). *)
+      (*         specialize (step_trans H11 H12) as H13. *)
+      (*         specialize (H1 l0 δ) as Z. *)
+      (*         destruct Z. subst. *)
+      (*         cbn in *. *)
+      (*         specialize (H14 l (env_snoc δ' (x, τ0) l0)). *)
+      (*         cbn in *. *)
+      (*         exists γfocus. *)
+      (*         apply (H14 γfocus). *)
+
+      (*         sound_steps_inversion. *)
+      (*         sound_simpl. *)
+
+      (*    dependent destruction H7. *)
+      (*    + cbn in *. *)
+      (*      specialize (H1 l δ). *)
+      (*      dependent destruction H1. *)
+      (*      cbn in *. *)
+      (*      specialize (H2 l (env_snoc δ (x, τ0) l)). *)
+      (*      specialize (H2 l H6 (env_snoc δ' (x, τ0) l) ). *)
+         admit.
+      (* rule_stm_if *)
+      - intros γfocus HP γframe Hsplit_γ.
+         sound_steps_inversion.
+         sound_simpl.
+         destruct (eval e δ); cbn in *.
+         * apply (IHtriple1 δ3 s4 H0 H1 γfocus (conj HP eq_refl) γframe Hsplit_γ).
+         * apply (IHtriple2 δ3 s4 H0 H1 γfocus (conj HP eq_refl) γframe Hsplit_γ).
+      (* rule_stm_if_backwards *)
+      - intros γfocus eqs γframe Hsplit_γ.
+        sound_steps_inversion.
+        sound_simpl.
+        destruct eqs as [HP1 HP2].
+        destruct (eval e δ); cbn in *.
+        + apply (IHtriple1 δ3 s4 H0 H1 γfocus (HP1 eq_refl) γframe Hsplit_γ).
+        + apply (IHtriple2 δ3 s4 H0 H1 γfocus (HP2 eq_refl) γframe Hsplit_γ).
+      (* rule_stm_seq *)
+      - intros γfocus HP γframe Hsplit_γ.
+         sound_steps_inversion.
+         sound_simpl.
+         destruct H5.
+         + sound_steps_inversion.
+           sound_simpl.
+           specialize (H2 δ0 δ' s' H10).
+         admit.
+      (* rule_stm_assert *)
+      - intros γfocus HP γframe Hsplit_γ.
+        sound_steps_inversion; try contradiction.
+        admit.
+      (* rule_stm_fail *)
+      - admit.
+      (* rule_stm_match_sum *)
+      - intros γfocus HP γframe Hsplit_γ.
+        sound_steps_inversion. sound_simpl.
+        destruct (eval e δ); cbn in *.
+        *
+          specialize (steps_inversion_let' H1 H0) as Z.
+          dependent destruction Z.
+          destruct_conjs.
+          progress (cbn in *).
+          exists γfocus.
+          specialize (step_trans H14 H15) as H16.
+          (* specialize (step_trans H15 Z). *)
+          cbn in *.
+
+          specialize (H3 l (env_cat H8 H9) H10 H11).
+          admit.
+        * exists γfocus. cbn in *.
+          sound_steps_inversion. sound_simpl.
+          destruct (eval e1 δ).
+        * exists γfocus.
+      1:{  }
+      1:{
+
+
+          apply (result_no_fail_inversion s' (fun v : Lit σ => Q v δ' γfocus')).
+          unfold ResultNoFail.
+
+      - cbn in *.
+      - cbn in *.
+        sound_steps_inversion.
+        dependent elimination triple.
+        2:{
+          exists γfocus.
+
+          cbn.
+          exists γl, γr.
+          split.
+          * apply Hsplit_γ.
+          * split.
+            ** apply HR.
+            ** dependent elimination t0.
+               remember (@rule_frame HProp _ Γ δ σ0 R P0 Q0 (stm_lit σ0 l) t0) as t.
+
+        + specialize (IHtriple l γ γ0 Heqγ0 γframe γfocus H2 (H γfocus H3)).
+          clear H3 H2 H.
+          destruct IHtriple as [γfocus' HQ'].
+          exists γfocus'. intuition.
+        + specialize (IHtriple l _ γfocus γr HP).
+          assert (forall (γ : RegStore) (hl hr : Heap),
+                     split (totalHeap γ) hl hr -> exists γl γr, totalHeap γl = hl
+                                                        /\ totalHeap γr = hr).
+          { intros.
+            unfold split in H.
+
+          specialize (IHtriple l γ γl).
+          assert (forall (R P : HProp) h, (R ✱ P) h -> P h).
+          { intros. destruct H as [hl [hr [_ [_ HP]]]]. apply HP.
+cbn in *.
+
+specialize (H2 γframe).
+
+
+        +
+          exists γfocus, γframe.
+          split.
+          * apply H3.
+          * eapply H1.
+            cbn in *.
+            specialize (H (totalHeap γfocus) H2).
+            specialize (IHtriple l γ γfocus H γframe H3).
+            destruct (
+            dependent destruction IHtriple.
+            dependent destruction H2.
+            dependent destruction H2.
+            apply H3.
+        (* generalize dependent γframe. *)
+        (* generalize dependent γfocus. *)
+        (* dependent induction triple. *)
+        (* + *)
+        (*   exists γfocus. *)
+        (*   eapply H1. *)
+        (*   cbn in *. *)
+        (*   specialize (H (totalHeap γfocus) H3). *)
+
+        (*   specialize (IHtriple l P' Q' eq_refl JMeq_refl JMeq_refl eq_refl JMeq_refl *)
+        (*               γframe γfocus H2 H). *)
+        (*   dependent elimination IHtriple. *)
+        (*   specialize (IHtriple l H) as z. *)
+        (*   dependent elimination z. *)
+
+
+
+eapply IHtriple.
+        dependent induction triple.
+        + exists γfocus.
+          specialize (IHtriple l PRE POST eq_refl ).
+
+          eapply H1.
+          eapply IHtriple.
+        dependent elimination triple.
+        + exists γfocus.
+          eapply l1.
+
+          destruct (@rule_consequence HProp _ Γ δ σ P P' Q Q' (stm_lit σ l) l0 l1 t).
+          *
+
+          eapply l1.
+          eapply l0.
+          dependent elimination t.
+          *
+        Focus 3.
+        cbn in *.
+        auto.
+        apply rule_stm_lit.
+        specialize (rule_stm_lit Γ δ τ l) as H.
+        cbn in H.
+        dependent destruction H.
+        + specialize (H2 l δ).
+
+        destruct (rule_stm).
+        specialize (POST l δ (totalHeap γ)) as t.
+        compute.
+
+        compute.
+        extensionality r.
+        compute.
+sound_simpl.
+        unfold HProp in *.
+        remember (totalHeap γ) as heap in *.
+        unfold Heap in *.
+        destruct (heap τ).
+        +
+        unfold ResultNoFail.
+        unfold totalHeap.
+        cbn.
+        eapply result_no_fail_inversion.
+      dependent induction H.
+      -
+      dependent destruction H1.
+
 
   (* The soundness proof needs to be carried out in terms of the logic interface *)
 
-
-  Definition sound_forward
-    (Γ : Ctx (𝑿 * Ty))
-    (σ : Ty)
-    (stm : Stm Γ σ)
-    (pre : LocalStore Γ -> A)
-    (post : LocalStore Γ -> Lit σ -> A)
-    (* (triple : Γ ⊢ ⦃ pre ⦄ stm ⦃ post ⦄) : *)
-    (triple : Triple Γ pre stm post) :
-    Valid (∀ γ1 μ1 δ1, ∃ stm' γ2 μ2 δ2,
-                !!(⟨ γ1 , μ1 , δ1 , stm ⟩ ---> ⟨ γ2 , μ2 , δ2 , stm' ⟩)).
 
     (* Proof. *)
     (*   destruct triple. *)
